saving work

src/Resolute_Logic.v
@@ -1,7 +1,8 @@
 (* Encoding of the RESOLUTE logic (and RESOLUTE to Copland translator) in coq *)
 
 Require Export String Maps.
-Require Export List.
+Require Export List EqClass.
+Require Import StructTactics.
 
 (* Generic ID Type -- for now, just make it nat *)
 Definition ID_Type := nat.
@@ -21,16 +22,80 @@ Inductive Term : Type :=
 | aspTerm : ASP_ID -> Term
 | seqTerm : Term -> Term -> Term.
 
+Fixpoint eqb_term `{EqClass ASP_ID} (t1 t2 : Term) : bool :=
+  match t1, t2 with
+  | emptyTerm, emptyTerm => true
+  | aspTerm a1, aspTerm a2 => eqb a1 a2
+  | seqTerm t11 t12, seqTerm t21 t22 =>
+    eqb_term t11 t21 && eqb_term t12 t22
+  | _, _ => false
+  end.
+
+Global Instance EqClass_Term : EqClass Term.
+eapply Build_EqClass with (eqb := eqb_term).
+induction x, y; ff;
+repeat rewrite PeanoNat.Nat.eqb_eq in *;
+ff;
+repeat rewrite Bool.andb_true_iff in *;
+ff; try split;
+repeat erewrite IHx1 in *;
+repeat erewrite IHx2 in *;
+ff.
+Defined.
+
 Inductive Evidence : Type := 
 | emptyE : Evidence
 | aspE : ASP_ID -> Evidence
 | seqE : Evidence -> Evidence -> Evidence.
+
+Fixpoint eqb_Evidence `{EqClass ASP_ID} (e1 e2 : Evidence) : bool :=
+  match e1, e2 with
+  | emptyE, emptyE => true
+  | aspE a1, aspE a2 => eqb a1 a2
+  | seqE e11 e12, seqE e21 e22 => 
+    eqb_Evidence e11 e21 && 
+    eqb_Evidence e12 e22
+  | _, _ => false
+  end.
+
+Global Instance EqClass_Evidence : EqClass Evidence.
+eapply Build_EqClass with (eqb := eqb_Evidence).
+induction x, y; ff;
+repeat rewrite PeanoNat.Nat.eqb_eq in *;
+ff;
+repeat rewrite Bool.andb_true_iff in *;
+ff; try split;
+repeat erewrite IHx1 in *;
+repeat erewrite IHx2 in *;
+ff.
+Defined.
 
 Inductive AppEvidence : Type := 
 | app_emptyE : AppEvidence
 | app_aspE : ASP_ID -> AppEvidence 
 | app_seqE : AppEvidence -> AppEvidence -> AppEvidence.
 
+Fixpoint eqb_AppEvidence `{EqClass ASP_ID} (e1 e2 : AppEvidence) : bool :=
+  match e1, e2 with
+  | app_emptyE, app_emptyE => true
+  | app_aspE a1, app_aspE a2 => eqb a1 a2
+  | app_seqE e11 e12, app_seqE e21 e22 => 
+    eqb_AppEvidence e11 e21 && 
+    eqb_AppEvidence e12 e22
+  | _, _ => false
+  end.
+
+Global Instance EqClass_AppEvidence : EqClass AppEvidence.
+eapply Build_EqClass with (eqb := eqb_AppEvidence).
+induction x, y; ff;
+repeat rewrite PeanoNat.Nat.eqb_eq in *;
+ff;
+repeat rewrite Bool.andb_true_iff in *;
+ff; try split;
+repeat erewrite IHx1 in *;
+repeat erewrite IHx2 in *;
+ff.
+Defined.
 (* Abstract system measurement -- vastly simplified simulation 
    of the Copland Virtual Machine (CVM) *)
 Fixpoint measure (t:Term) : Evidence := 
@@ -55,57 +120,220 @@ Inductive Resolute : Type :=
   | R_And (G1 : Resolute) (G2 : Resolute)
   | R_Or (G1 : Resolute) (G2 : Resolute)
   | R_Imp (G1 : Resolute) (G2 : Resolute)
-  | R_Forall (l : list Target_ID)  (G : Target_ID -> Resolute)
-  | R_Exists (l : list Target_ID) (G : Target_ID -> Resolute).
+  | R_Forall (l : list Target_ID) (fn : string)
+    (* (G : Target_ID -> Resolute) *)
+  | R_Exists (l : list Target_ID) (fn : string).
+  (* (G : Target_ID -> Resolute). *)
+
+Fixpoint eqb_Resolute `{EqClass string, EqClass (list Target_ID)} (r1 r2 : Resolute) : bool :=
+  match r1, r2 with
+  | R_False, R_False => true
+  | R_True, R_True => true
+  | R_Goal t1, R_Goal t2 => eqb t1 t2
+  | R_And g11 g12, R_And g21 g22 =>
+    eqb_Resolute g11 g21 && eqb_Resolute g12 g22
+  | R_Or g11 g12, R_Or g21 g22 =>
+    eqb_Resolute g11 g21 && eqb_Resolute g12 g22
+  | R_Imp g11 g12, R_Imp g21 g22 =>
+    eqb_Resolute g11 g21 && eqb_Resolute g12 g22
+  | R_Forall l1 f1, R_Forall l2 f2 =>
+    eqb f1 f2 && eqb l1 l2
+  | R_Exists l1 f1, R_Exists l2 f2 =>
+    eqb f1 f2 && eqb l1 l2
+  | _, _ => false
+  end.
+
+Instance EqClass_Resolute `{EqClass string, EqClass (list Target_ID)}
+  : EqClass Resolute.
+eapply Build_EqClass with (eqb := eqb_Resolute).
+induction x, y; ff;
+repeat rewrite PeanoNat.Nat.eqb_eq in *;
+ff;
+repeat rewrite Bool.andb_true_iff in *;
+ff; try split;
+repeat erewrite IHx1 in *;
+repeat erewrite IHx2 in *;
+ff;
+repeat rewrite eqb_eq in *; ff.
+Defined.
 
 Definition Assumption := Resolute.
 Definition Assumptions := list (Assumption).
 
 Record Model := {
-  conc : Target_ID -> Term ;
-  spec : Target_ID -> list AppEvidence
+  fns   : MapC string (Target_ID -> Resolute) ;
+  conc  : Target_ID -> Term ;
+  spec  : Target_ID -> (AppEvidence -> Prop) ;
+  (* list AppEvidence *)
 }.
 
-Fixpoint res_to_copland (M : Model) (r:Resolute) : Term * (AppEvidence -> Prop) :=
+Fixpoint res_to_copland `{Heq : EqClass Resolute} (M : Model) 
+    (A : Assumptions) (r:Resolute) {struct r}
+    : Term * (AppEvidence -> Prop) :=
+  (* check r \in assumptions *)
+  if (in_dec (EqClass_impl_DecEq _) r A)
+  then (emptyTerm, fun e => True)
+  else
   match r with 
   | R_False => (emptyTerm, fun e => False)
 
   | R_True => (emptyTerm, fun e => True)
 
-  | (R_Goal tid) => (conc M tid, fun e => In e (spec M tid))
+  | (R_Goal tid) => (conc M tid, spec M tid)
+  (* fun e => In e (spec M tid)) *)
 
   | R_And r1 r2 => 
-    let '(t1, pol1) := res_to_copland M r1 in
-    let '(t2, pol2) := res_to_copland M r2 in
-    (seqTerm t1 t2, fun e => pol1 e /\ pol2 e)
+    let '(t1, pol1) := res_to_copland M A r1 in
+    let '(t2, pol2) := res_to_copland M A r2 in
+    (seqTerm t1 t2, fun e => 
+      match e with
+      | app_seqE e1 e2 => pol1 e1 /\ pol2 e2
+      | _ => False
+      end)
 
   | R_Or r1 r2 => 
-    let '(t1, pol1) := res_to_copland M r1 in
-    let '(t2, pol2) := res_to_copland M r2 in
-    (seqTerm t1 t2, fun e => pol1 e \/ pol2 e)
+    let '(t1, pol1) := res_to_copland M A r1 in
+    let '(t2, pol2) := res_to_copland M A r2 in
+    (seqTerm t1 t2, fun e => 
+      match e with
+      | app_seqE e1 e2 => pol1 e1 \/ pol2 e2
+      | _ => False
+      end)
 
   | R_Imp r1 r2 => 
-    let '(t1, pol1) := res_to_copland M r1 in
-    let '(t2, pol2) := res_to_copland M r2 in
-    (seqTerm t1 t2, fun e => pol1 e -> pol2 e)
+    let '(t1, pol1) := res_to_copland M A r1 in
+    let '(t2, pol2) := res_to_copland M (r1 :: A) r2 in
+    (seqTerm t1 t2, fun e => 
+      match e with
+      | app_seqE e1 e2 => pol1 e1 -> pol2 e2
+      | _ => False
+      end)
 
-  | R_Forall l pred => 
+  | R_Forall l fnName => 
     (* forall x \in l, do pred l *)
-    let list_tpols := map (fun x => res_to_copland M (pred x)) l in
-    fold_left (fun x y => (seqTerm (fst x) (fst y), fun e => (snd x) e /\ (snd y) e)) list_tpols (emptyTerm, fun e => True)
+    match map_get (fns M) fnName with
+    | None => (emptyTerm, fun e => False)
+    | Some fn =>
+    let list_tpols := map (fun x => res_to_copland M A (fn x)) l in
+    fold_left (fun x y => (seqTerm (fst x) (fst y), (fun e => 
+      match e with
+      | app_seqE e1 e2 => (snd x) e1 /\ (snd y) e2
+      | _ => False
+      end))) list_tpols (emptyTerm, fun e => True)
+    end
 
-  | R_Exists l pred => 
+  | R_Exists l fnName => 
     (* exists x \in l, do pred l *)
-    let list_tpols := map (fun x => res_to_copland M (pred x)) l in
-    fold_left (fun x y => (seqTerm (fst x) (fst y), fun e => (snd x) e \/ (snd y) e)) list_tpols (emptyTerm, fun e => False)
+    match map_get (fns M) fnName with
+    | None => (emptyTerm, fun e => False)
+    | Some fn =>
+    let list_tpols := map (fun x => res_to_copland M A (fn x)) l in
+    fold_left (fun x y => (seqTerm (fst x) (fst y), (fun e => 
+      match e with
+      | app_seqE e1 e2 => (snd x) e1 \/ (snd y) e2
+      | _ => False
+      end))) list_tpols (emptyTerm, fun e => False)
+    end
   end.
- 
+
+Lemma thing : forall A B,
+  {A} + {~ A} ->
+  {B} + {~ B} ->
+  {A -> B} + {~ (A -> B)}.
+Proof.
+  intuition.
+Qed.
+
+Lemma thing2 : forall A B,
+  A \/ ~ A ->
+  B \/ ~ B ->
+  (A -> B) \/ (~ (A -> B)).
+Proof.
+  intuition.
+Qed.
+
+Theorem fold_left_ind : forall A B (f : A -> B -> A) l start P P',
+  P start ->
+  (forall a b, P a -> P' b -> P (f a b)) ->
+  (forall b, In b l -> P' b) ->
+  P (fold_left f l start).
+Proof.
+  induction l; ff.
+  eapply IHl; ff.
+Qed.
+
+(* NOTE: If we can get something stronger out of this,
+we will be able to prove DECIDABILITY, stronger than LEM *)
+Theorem map_spec : forall A B (f : A -> B) l b,
+  In b (map f l) ->
+  exists a, f a = b.
+Proof.
+  induction l; ff.
+Qed.
+
+(*
+
+Theorem LEM_appr_proc : forall M r t pol,
+  res_to_copland M r = (t, pol) ->
+  pol (appraise (measure t)) \/ ~ pol (appraise (measure t)).
+Proof.
+  induction r; simpl in *; ff.
+  - edestruct in_dec;
+    try (eapply EqClass_impl_DecEq; eapply EqClass_AppEvidence);
+    ff.
+  - try pose proof (IHr1 _ _ eq_refl);
+    try pose proof (IHr2 _ _ eq_refl);
+    destruct H, H0; ff;
+    right; intros HC; ff.
+  - try pose proof (IHr1 _ _ eq_refl);
+    try pose proof (IHr2 _ _ eq_refl);
+    destruct H, H0; ff;
+    right; intros HC; ff.
+  - try pose proof (IHr1 _ _ eq_refl);
+    try pose proof (IHr2 _ _ eq_refl);
+    ff.
+    eapply thing2; ff.
+  - (* need lemma that says if 
+    P start ->
+    (forall fn x, P x -> P (fn x)) ->
+    P (fold_left start fn)
+  *)
+    pose proof (fold_left_ind (Term * (AppEvidence  -> Prop)) _ (fun x y =>
+      (seqTerm (fst x) (fst y), (fun e => match e with
+        | app_seqE e1 e2 => snd x e1 /\ snd y e2
+        | _ => False
+      end))) (map (fun x => res_to_copland M (G x)) l) (emptyTerm, fun _ => True) (fun '(t', pol') => pol' (appraise (measure t')) \/ ~ pol'(appraise (measure t'))) (fun '(t', pol') => pol' (appraise (measure t')) \/ ~ pol'(appraise (measure t')))).
+    simpl in *.
+    setoid_rewrite H0 in X.
+    eapply X; ff.
+    * destruct X1, X0; ff;
+      right; intros HC; ff. 
+    * eapply map_spec in H1;
+      ff.
+  - pose proof (fold_left_ind (Term * (AppEvidence  -> Prop)) _ (fun x y =>
+      (seqTerm (fst x) (fst y), (fun e => match e with
+        | app_seqE e1 e2 => snd x e1 \/ snd y e2
+        | _ => False
+      end))) (map (fun x => res_to_copland M (G x)) l) (emptyTerm, fun _ => True) (fun '(t', pol') => pol' (appraise (measure t')) \/ ~ pol'(appraise (measure t'))) (fun '(t', pol') => pol' (appraise (measure t')) \/ ~ pol'(appraise (measure t')))).
+    simpl in *.
+    setoid_rewrite H0 in X.
+    eapply X; ff.
+    * right; intros HC; ff.
+    * eapply map_spec in H1;
+      ff. 
+Qed.
+*)
 
 Inductive Reval : Assumptions -> Resolute -> Prop :=
   | Reval_L : forall A G,
     In R_False A -> Reval (A) G
   | Reval_R : forall A,
     Reval A R_True
+  | Reval_Back : forall G A a',
+    In a' A ->
+    Reval (a' :: A) G ->
+    Reval A G
+    (* In G A -> Reval A G *)
   | Reval_And : forall A G1 G2,
     Reval A G1 -> Reval A G2 -> Reval A (R_And G1 G2)
   | Reval_Or_L : forall A G1 G2,
@@ -126,12 +354,260 @@ Inductive Reval : Assumptions -> Resolute -> Prop :=
         In v tp -> 
         Reval A (pred v)) ->
       Reval A (R_Exists tp pred).
+Global Hint Constructors Reval : core.
 
-Theorem res_to_copland_sound : forall (m:Model) (r:Resolute),
-  (forall t pol, res_to_copland m r=(t,pol) -> pol (appraise (measure t)))
-  <->
-  (forall a, Reval a r).
+(* Definition consistent (A:Assumptions) : Prop :=
+  forall G, In G A -> 
+    Reval A G.
+  forall G, Reval A G -> G = R_True.
+
+Lemma reval_or_spec : forall A,
+  () *)
+
+Lemma reval_or_spec : forall A G1 G2,
+  Reval A (R_Or G1 G2) <->
+  Reval A G1 \/ Reval A G2.
 Proof.
+  split; intros; ff;
+  prep_induction H;
+  induction H; ff;
+  pose proof (IHReval _ _ eq_refl); ff.
+Qed.
+
+Lemma reval_and_spec : forall A G1 G2,
+  Reval A (R_And G1 G2) <->
+  Reval A G1 /\ Reval A G2.
+Proof.
+  split; intros; ff;
+  prep_induction H;
+  induction H; ff;
+  pose proof (IHReval _ _ eq_refl); ff.
+Qed.
+
+(*
+
+Theorem Reval_ext : forall G A A',
+  (forall a, In a A -> In a A') ->
+  Reval A G ->
+  Reval A' G.
+Proof.
+  induction G; ff;
+  try (pose proof (IHG1 _ _ H);
+    pose proof (IHG2 _ _ H); ff).
+  - generalize dependent A'.
+    induction H0; ff.
+    * eapply IHReval; ff. 
+    * eapply Reval_Imp.
+      eapply IHReval; ff.
+    * eapply Reval_Exists.
+      eexists; ff.
+      eapply H in H1.
+      clear H.
+      set (X := pred x) in *.
+
+    *  
+    invc H0;
+    try (eapply Reval_L; ff; fail);
+    try (eapply Reval_Back; ff; fail).
+    eapply Reval_Back.
+    eapply 
+  - invc H0;
+    try (eapply Reval_L; ff; fail);
+    try (eapply Reval_Refl; ff; fail).
+    eapply Reval_Imp.
+    eapply IHG2;
+    try (eapply H3); ff.
+  - invc H1;
+    try (eapply Reval_L; ff; fail);
+    try (eapply Reval_Refl; ff; fail).
+    eapply Reval_Forall;
+    ff.
+  - invc H1;
+    try (eapply Reval_L; ff; fail);
+    try (eapply Reval_Refl; ff; fail).
+    eapply Reval_Exists;
+    ff.
+Qed.
+*)
+
+Lemma in_r_false_A : forall l,
+  {In R_False l} + {~ (In R_False l)}.
+Proof.
+  induction l; ff.
+  destruct IHl; ff. 
+  destruct a; ff;
+  right; intros HC; ff.
+Qed.
+
+Lemma in_r_goal_A : forall t l,
+  {In (R_Goal t) l} + {~ (In (R_Goal t) l)}.
+Proof.
+  induction l; ff.
+  destruct IHl; ff. 
+  destruct a; ff;
+  try (right; intros HC; ff; fail);
+  destruct (PeanoNat.Nat.eq_dec t T);
+  ff; right; intros HC; ff.
+Qed.
+
+(* 
+
+Theorem LEM_reval : forall A r,
+  Reval A r \/ ~ Reval A r.
+Proof.
+  induction r; ff.
+  - destruct (in_r_false_A A); ff.
+    right; intros HC.
+    inversion HC; ff.
+  - destruct (in_r_goal_A T A); ff.
+    destruct (in_r_false_A A); ff.
+    right; intros HC.
+    inversion HC; ff.
+  - destruct IHr1, IHr2; ff;
+    right; intros HC; 
+    inversion HC; ff.
+    * left; ff.
+*)
+
+Axiom in_spec_reval : forall M T,
+  spec M T (appraise (measure (conc M T))) <->
+  (* In (appraise (measure (conc m T))) (spec m T) <-> *)
+  (forall a, Reval a (R_Goal T)).
+
+(*
+
+Lemma reval_trans : forall A r1,
+  Reval A r1 ->
+  forall r2,
+  Reval (r1 :: A) r2 ->
+  Reval A r2.
+Proof.
+  intros A r1 H.
+  induction H; ff. 
+  - admit. 
+  - admit. 
+  - admit. 
+  - induction r2; ff;
+    invc H0; ff.
+    * invc H0; ff. 
+    *  
+  induction r1; ff.
+  - clear H.
+    induction H0; ff.
+    *  
+  intros A r1 H.
+  induction H; ff.
+  - invc H; eauto. 
+
+Lemma reval_cons : forall A r A' A'',
+  Reval A r ->
+  Reval (A' ++ A ++ A'') r.
+Proof.
+  induction r; ff;
+  try (invc H; try (eapply Reval_L; repeat rewrite in_app_iff; ff; fail);
+    try (eapply Reval_Refl; repeat rewrite in_app_iff; ff; fail); ffa; fail).
+  - 
+    invc H; try (eapply Reval_L; repeat rewrite in_app_iff; ff; fail);
+    try (eapply Reval_Refl; repeat rewrite in_app_iff; ff; fail).
+    eapply Reval_Imp; ff.
+    * eapply Reval_L; ff.
+    *  
+*)
+Axiom decidable_appr_proc : forall P t,
+  {P (appraise (measure t))} + {~ P (appraise (measure t))}.
+
+Theorem res_to_copland_sound : forall (m:Model) (r:Resolute) t pol,
+  res_to_copland m r = (t,pol) -> 
+  pol (appraise (measure t)) ->
+  forall A,
+
+  (* forall A,
+    (forall a t' pol', 
+      In a A ->
+      res_to_copland m a = (t', pol') -> 
+      pol' (appraise (measure t'))
+    ) -> *)
+  Reval A r.
+Proof.
+  induction r; simpl in *; intuition;
+  repeat find_eapply_hyp_hyp;
+  repeat find_injection; simpl in *;
+  intuition.
+  - eapply in_spec_reval; eauto. 
+  - repeat break_match; repeat find_injection;
+    simpl in *; intuition.
+    pose proof (IHr1 _ _ eq_refl H).
+    pose proof (IHr2 _ _ eq_refl H1).
+    eauto.
+    (* pose proof (IHr1 _ _ eq_refl H _ H1).
+    pose proof (IHr2 _ _ eq_refl H2 _ H1).
+    eauto. *)
+  - repeat break_match; repeat find_injection;
+    simpl in *; intuition;
+    try pose proof (IHr1 _ _ eq_refl H);
+    try pose proof (IHr2 _ _ eq_refl H2);
+    eauto.
+  - repeat break_match; repeat find_injection;
+    simpl in *; intuition.
+    try pose proof (IHr1 _ _ eq_refl H);
+    try pose proof (IHr2 _ _ eq_refl H2);
+    eauto. 
+    destruct (decidable_appr_proc P t0);
+    destruct (decidable_appr_proc P0 t1);
+    eauto.
+    admit.
+  - pose proof (fold_left_ind _ _ (fun x y : Term * (AppEvidence -> Prop) => (seqTerm (fst x) (fst y),
+fun e : AppEvidence => match e with
+| app_seqE e1 e2 => snd x e1 /\ snd y e2
+| _ => False
+end)) (map (fun x => res_to_copland m (G x)) l) (emptyTerm, (fun _ => True)) (fun '(t, pol) => pol (appraise (measure t))) (fun '(t, pol) => pol (appraise (measure t)))); simpl in *.
+repeat find_rewrite.
+simpl in *.
+intuition.
+  eapply Reval_Forall.
+  intuition.
+  eapply H; ff.
+    intros.
+    eapply H0; eauto.
+  pose proof (fold_left_ind).
+    pose proof thing. 
+    pose proof thing2.
+    intuition; ff.
+    * pose proof (IHr1 _ _ eq_refl p _ H1).
+      find_eapply_hyp_hyp; eauto.
+      eapply Reval_Imp.
+      eapply Reval_Refl.
+  -  
+    eauto.
+    simpl in *.
+    unfold measure in H.
+    simpl in *.
+
+
+  try (pose proof (H _ _ eq_refl); simpl in *; intuition).
+  - eapply Reval_R. 
+  - eapply in_spec_reval in H1; eauto.
+  - repeat break_match; intuition. 
+  split.
+  - induction r; simpl in *; intuition;
+    try pose proof (H _ _ eq_refl);
+    simpl in *; intuition.
+    * eapply Reval_R.
+    * eapply in_spec_reval; eauto. 
+    * eapply Reval_And;
+      repeat break_match.
+      ** pose proof (H _ _ eq_refl); simpl in *;
+        intuition. 
+        pose proof (IHr1 t P).
+        eapply IHr2 in H2.
+  induction r.
+  -  
+  - pose proof (H _ _ eq_refl). 
+    simpl in *; intuition.
+  - repeat find_injection. 
+    pose proof (H nil); invc H0;
+    invc H1.
+  -  
   intros. split; intros H.
   - induction r.
     (* R_False: solved *)
