src/FOL.v
@@ -1,0 +1,245 @@
+Inductive testT := testC.
+
+Require Import StructTactics.
+Require Import String List Lia.
+Import ListNotations.
+
+Definition Forall' {A : Type} (P : A -> Prop) : list A -> Prop :=
+  fix F l :=
+    match l with
+    | nil => True
+    | x :: l' => P x /\ F l'
+    end.
+
+Theorem Forall'_spec : forall A P (l : list A),
+  Forall' P l <->
+  (forall a, In a l -> P a).
+Proof.
+  induction l; ff.
+Qed.
+
+Definition Exists' {A : Type} (P : A -> Prop) : list A -> Prop :=
+  fix F l :=
+    match l with
+    | nil => False
+    | x :: l' => P x \/ F l'
+    end.
+
+Theorem Exists'_spec : forall A P (l : list A),
+  Exists' P l <->
+  (exists a, In a l /\ P a).
+Proof.
+  induction l; ff.
+  - rewrite IHl in H0; ff. 
+  - assert (exists x, In x l /\ P x) by ff.
+    rewrite <- IHl in H; ff.
+Qed.
+
+Inductive vec (A : Type) : nat -> Type :=
+| vnil : vec A 0
+| vcons : A -> forall n, vec A n -> vec A (S n).
+Arguments vnil {A}.
+Arguments vcons {A} _ {n} _.
+Notation "[||]" := vnil (at level 150).
+Notation "[| x ; .. ; y |]" := (vcons x .. (vcons y vnil) ..) (at level 160).
+Notation "x |:: v" := (vcons x v) (at level 60, right associativity).
+
+Example vec_ex1 : vec nat 3 := [| 1 ; 2 ; 3 |].
+Example vec_ex2 : vec nat 3 := 1 |:: 2 |:: 3 |:: vnil.
+Example vec_ex_eq1 : vec_ex1 = vec_ex2 := eq_refl.
+
+Module Type FOL_Language.
+  (* NOTE: Constants are considered 0 argument Functions! *)
+  Parameter Preds : list (string * nat).
+
+  Parameter Funcs : list (string * nat).
+
+  Inductive Logicals :=
+  | Log_neg 
+  | Log_conj
+  | Log_disj
+  | Log_cond
+  | Log_univ
+  | Log_exists
+  | Log_bot
+  | Log_eq
+  | Log_var : string -> Logicals.
+
+  Inductive Symbols :=
+  | Sym_pred : { x | In x Preds } -> list Symbols -> Symbols
+  | Sym_func : { x | In x Funcs } -> list Symbols -> Symbols
+  | Sym_log : Logicals -> Symbols
+  | Sym_comma.
+
+End FOL_Language.
+
+Module FOL.
+
+  Declare Module L : FOL_Language.
+
+  Unset Positivity Checking.
+
+  Inductive Term :=
+  | T_var : string -> Term
+  | T_func : { x | In (fst x) L.Funcs /\ @length Term (snd x) = snd (fst x) } -> Term.
+
+  Print map.
+
+  Definition fancy_map {A : Type} {P : A -> Prop} (fn : A -> A) (projFn : { x | P x } -> list A) : { x | P x } -> { x | P x }.
+    refine (fun l =>
+      match l with
+      | exist _ (p', nil) PV => exist _ (p', nil) PV
+      | exist _ (p', (x :: l)) PV => exist _ (p', (fn x :: map fn l)) _
+      end).
+    simpl in *; intuition;
+    erewrite map_length; ff.
+  Defined.
+
+  Fixpoint closed_term (t : Term) :=
+    match t with
+    | T_var _ => False
+    | T_func l => Forall' closed_term (snd (proj1_sig l))
+    end.
+
+  Inductive Formula :=
+  | F_bot : Formula
+  | F_pred : { x | In (fst x) L.Preds /\ @length Term (snd x) = snd (fst x) } -> Formula
+  | F_eq : Term -> Term -> Formula
+  | F_not : Formula -> Formula
+  | F_and : Formula -> Formula -> Formula
+  | F_or : Formula -> Formula -> Formula
+  | F_impl : Formula -> Formula -> Formula
+  | F_forall : string -> Formula -> Formula
+  | F_exists : string -> Formula -> Formula.
+
+  Definition syntactic_eq (s1 s2 : list L.Symbols) :=
+    s1 = s2.
+
+  Fixpoint proper_subformula (f : Formula) : list Formula :=
+    match f with
+    | F_bot => nil
+    | F_pred l => nil
+    | F_eq _ _ => nil
+    | F_not f' => f' :: proper_subformula f'
+    | F_and f1 f2 => f1 :: f2 :: proper_subformula f1 ++ proper_subformula f2
+    | F_or f1 f2 => f1 :: f2 :: proper_subformula f1 ++ proper_subformula f2
+    | F_impl f1 f2 => f1 :: f2 :: proper_subformula f1 ++ proper_subformula f2
+    | F_forall _ f' => f' :: proper_subformula f'
+    | F_exists _ f' => f' :: proper_subformula f'
+    end.
+
+  Definition subformula (f : Formula) : list Formula :=
+    f :: proper_subformula f.
+
+  Fixpoint vars_term (t : Term) : list string :=
+    match t with
+    | T_var x => [x]
+    | T_func l => flat_map vars_term (snd (proj1_sig l))
+    end.
+
+  Fixpoint free_vars_term (t : Term) : list string :=
+    match t with
+    | T_var x => [x]
+    | T_func l => flat_map free_vars_term (snd (proj1_sig l))
+    end.
+
+  Fixpoint vars_formula (f : Formula) : list string :=
+    match f with
+    | F_bot => nil
+    | F_pred l => flat_map vars_term (snd (proj1_sig l))
+    | F_eq t1 t2 => vars_term t1 ++ vars_term t2
+    | F_not f' => vars_formula f'
+    | F_and f1 f2 => vars_formula f1 ++ vars_formula f2
+    | F_or f1 f2 => vars_formula f1 ++ vars_formula f2
+    | F_impl f1 f2 => vars_formula f1 ++ vars_formula f2
+    | F_forall x f' => vars_formula f'
+    | F_exists x f' => vars_formula f'
+    end.
+
+  Fixpoint free_vars_formula (f : Formula) : list string :=
+    match f with
+    | F_bot => nil
+    | F_pred l => flat_map free_vars_term (snd (proj1_sig l))
+    | F_eq t1 t2 => free_vars_term t1 ++ free_vars_term t2
+    | F_not f' => free_vars_formula f'
+    | F_and f1 f2 => free_vars_formula f1 ++ free_vars_formula f2
+    | F_or f1 f2 => free_vars_formula f1 ++ free_vars_formula f2
+    | F_impl f1 f2 => free_vars_formula f1 ++ free_vars_formula f2
+    | F_forall x f' => remove string_dec x (free_vars_formula f')
+    | F_exists x f' => remove string_dec x (free_vars_formula f')
+    end.
+
+  Definition var_bound_term (t : Term) : list string :=
+    let vars := vars_term t in
+    let free_vars := free_vars_term t in
+    filter (fun x => if In_dec string_dec x free_vars then false else true) vars.
+
+  Definition var_bound_formula (f : Formula) : list string :=
+    let vars := vars_formula f in
+    let free_vars := free_vars_formula f in
+    filter (fun x => if In_dec string_dec x free_vars then false else true) vars.
+
+  Definition sentence (f : Formula) :=
+    free_vars_formula f = nil.
+
+  Definition subst_term (x : string) (t' : Term) : Term -> Term :=
+    fix subst_term t :=
+      match t with
+      | T_var x' => if string_dec x x' then t' else t
+      | T_func l => T_func (fancy_map subst_term l)
+      end.
+  destruct l, x0; simpl in *.
+  set (l' := map subst_term l).
+  pose proof (@exist).
+  assert (In p L.Funcs /\ length l' = (snd p)). {
+    intuition.
+    subst l'.
+    rewrite map_length.
+    eauto.
+  }
+  eapply (T_func (@exist _ (fun x0 => In (fst x0) L.Funcs /\ length (snd x0) = snd (fst x0)) (p, l') H)). 
+  Defined.
+  eapply H0.
+
+
+
+  destruct t.
+  - eapply (if string_dec x s then t' else T_var s). 
+  - destruct s, x0; simpl in *.
+    set (l' := map )
+    pose 
+    match t with
+    | T_var x' => if string_dec x x' then t' else t
+    | T_func l => T_func (exist _ (fst (proj1_sig l), map (subst_term x t') (snd (proj1_sig l)) _) _)
+    end.
+
+  Definition subst_term (x : string) (t' : Term) : Term -> Term :=
+    fix subst_term t :=
+      match t with
+      | T_var x' => if string_dec x x' then t' else t
+      | T_func l => T_func (map subst_term (snd (proj1_sig l)))
+      end.
+
+  Definition subst_formula (x : string) (t' : Term) : Formula -> Formula :=
+    fix subst_formula f :=
+      match f with
+      | F_bot => F_bot
+      | F_pred p l => F_pred p (map (subst_term x t') l)
+      | F_eq t1 t2 => F_eq (subst_term x t' t1) (subst_term x t' t2)
+      | F_not f1 => F_not (subst_formula f1)
+      | F_and f1 f2 => F_and (subst_formula f1) (subst_formula f2)
+      | F_or f1 f2 => F_or (subst_formula f1) (subst_formula f2)
+      | F_impl f1 f2 => F_impl (subst_formula f1) (subst_formula f2)
+      | F_forall x' f1 => if string_dec x x' then F_forall x' f1 else F_forall x' (subst_formula f1)
+      | F_exists x' f1 => if string_dec x x' then F_exists x' f1 else F_exists x' (subst_formula f1)
+      end.
+
+  Record Model := {
+    Domain      : Type;
+    ConstInterp : string -> Domain;
+    FuncInterp  : { x | In x L.Funcs } -> list Domain -> Domain;
+    Relations : string -> list Domain -> Prop
+  }.
+
+Inductive Term :=
+| Var : string -> Term
